introduce kernel state

kernel-template/coq/Kernel.v
@@ -7,6 +7,11 @@ Require Import Turn.
 Open Local Scope hprop_scope.
 Open Local Scope stsepi_scope.
 
+Record kstate : Set :=
+  mkst { c : chan
+       ; ktr : [Trace]
+       }.
+
 Inductive KTrace : Trace -> Prop :=
 | KT_init :
   KTrace nil
@@ -15,43 +20,57 @@ Inductive KTrace : Trace -> Prop :=
   KTrace tr ->
   KTrace (SendMsgs c (protocol m) ++ RecvMsg c m ++ tr).
 
-Definition kloop:
-  forall (c : chan) (tr : [Trace]),
-  STsep (tr ~~ traced tr * bound c * [KTrace tr])
-        (fun (tr' : [Trace]) => tr' ~~ traced tr' * bound c * [KTrace tr']).
+Definition kstate_inv s : hprop :=
+  tr :~~ ktr s in
+  traced tr * [KTrace tr] * bound (c s).
+
+Definition kbody:
+  forall s,
+  STsep (kstate_inv s)
+        (fun s' => kstate_inv s').
 Proof.
-  intros; refine (
-    Fix2
-      (fun (_ : unit) (tr : [Trace]) => tr ~~ traced tr * bound c * [KTrace tr])
-      (fun (_ : unit) (tr tr' : [Trace]) => tr' ~~ traced tr' * bound c * [KTrace tr'])
-      (fun self (_ : unit) (tr : [Trace]) =>
-        req <- turn c
-          tr <@>
-          (tr ~~ [KTrace tr]);
-        tr' <- self tt
-          (tr ~~~ SendMsgs c (protocol req) ++ RecvMsg c req ++ tr) <@>
-          (tr ~~ [KTrace tr]);
-        {{ Return  tr' }})
-      tt tr
+  unfold kstate_inv; intros [c tr];
+  refine (
+    req <- turn c
+      tr <@>
+      (tr ~~ [KTrace tr]);
+    {{ Return (mkst c (tr ~~~ SendMsgs c (protocol req) ++ RecvMsg c req ++ tr)) }}
   );
   sep fail auto.
-  apply himp_pure'.
-  constructor; auto.
+  apply himp_pure'; constructor; auto.
 Qed.
 
-Axiom c : chan.
+Definition kloop:
+  forall s,
+  STsep (kstate_inv s)
+        (fun s' => kstate_inv s').
+Proof.
+  intros; refine (
+    Fix
+      (fun s => kstate_inv s)
+      (fun s s' => kstate_inv s')
+      (fun self s =>
+        s <- kbody s;
+        s <- self s;
+        {{ Return s }}
+      )
+    s
+  );
+  sep fail auto.
+Qed.
+
+Axiom dummy : chan.
 
 Definition main:
   forall (_ : unit),
-  STsep (traced nil * bound c)
-        (fun (tr : [Trace]) => tr ~~ traced tr * bound c * [KTrace tr]).
+  STsep (traced nil * bound dummy)
+        (fun s' => kstate_inv s').
 Proof.
   intros; refine (
-    tr' <- kloop c
-      [nil];
-    {{ Return tr' }}
+    s' <- kloop (mkst dummy [nil]);
+    {{ Return s' }}
   );
+  unfold kstate_inv;
   sep fail auto.
-  apply himp_pure'.
-  constructor; auto.
+  apply himp_pure'; constructor; auto.
 Qed.
